src/ElimFunc3.v
@@ -5,7 +5,7 @@ Require Import Utopia.
 Require Import Monads.
 Require Import ListLemmas.
 Require Import Psatz.
-Require HigherValue.
+Require Import HigherValue.
 
 
 (* Uses the same syntax as ElimFunc2 *)
@@ -15,14 +15,22 @@ Require Export ElimFunc2.
 (* Continuation-based step relation *)
 
 Inductive state :=
-| Run (e : expr) (l : list expr) (k : expr -> state)
-| Stop (e : expr).
+| Run (e : expr) (l : list value) (k : value -> state)
+| Stop (e : value).
 
-Definition state_expr s :=
-    match s with
-    | Run e _ _ => e
-    | Stop e => e
-    end.
+(* Definition state_expr s := *)
+(*     match s with *)
+(*     | Run e _ _ => e *)
+(*     | Stop e => e *)
+(*     end. *)
+
+Definition unwrap (e : expr) :=
+  match e with
+  | Value v => Some v
+  | _ => None
+  end.
+
+Definition unwrap_list := map_partial unwrap.
 
 Inductive sstep (E : env) : state -> state -> Prop :=
 | SArg : forall l k v,
@@ -31,48 +39,41 @@ Inductive sstep (E : env) : state -> state -> Prop :=
 | SUpVar : forall n l k v,
         nth_error l (S n) = Some v ->
         sstep E (Run (UpVar n) l k) (k v)
-
 | SCloseStep : forall fname vs e es l k,
-        Forall value vs ->
-        ~ value e ->
-        sstep E (Run (Close fname (vs ++ [e] ++ es)) l k)
-                (Run e l (fun v => Run (Close fname (vs ++ [v] ++ es)) l k))
-| SCloseDone : forall fname vs l k,
-        Forall value vs ->
-        sstep E (Run (Close fname vs) l k) (k (Close fname vs))
-
+        Forall is_value vs ->
+        ~ is_value e ->
+        sstep E (Run (MkClose fname (vs ++ [e] ++ es)) l k)
+                (Run e l (fun v => Run (MkClose fname (vs ++ [Value v] ++ es)) l k))
+| SCloseDone : forall fname es vs l k,
+        unwrap_list es = Some vs ->
+        sstep E (Run (MkClose fname es) l k) (k (Close fname vs))
 | SConstrStep : forall fname vs e es l k,
-        Forall value vs ->
-        ~ value e ->
-        sstep E (Run (Constr fname (vs ++ [e] ++ es)) l k)
-                (Run e l (fun v => Run (Constr fname (vs ++ [v] ++ es)) l k))
-| SConstrDone : forall fname vs l k,
-        Forall value vs ->
-        sstep E (Run (Constr fname vs) l k) (k (Constr fname vs))
-
+        Forall is_value vs ->
+        ~ is_value e ->
+        sstep E (Run (MkConstr fname (vs ++ [e] ++ es)) l k)
+                (Run e l (fun v => Run (MkConstr fname (vs ++ [Value v] ++ es)) l k))
+| SConstrDone : forall fname es vs l k,
+        unwrap_list es = Some vs ->
+        sstep E (Run (MkConstr fname es) l k) (k (Constr fname vs))
 | SCallL : forall e1 e2 l k,
-        ~ value e1 ->
+        ~ is_value e1 ->
         sstep E (Run (Call e1 e2) l k)
-                (Run e1 l (fun v => Run (Call v e2) l k))
+                (Run e1 l (fun v => Run (Call (Value v) e2) l k))
 | SCallR : forall e1 e2 l k,
-        value e1 ->
-        ~ value e2 ->
+        is_value e1 ->
+        ~ is_value e2 ->
         sstep E (Run (Call e1 e2) l k)
-                (Run e2 l (fun v => Run (Call e1 v) l k))
+                (Run e2 l (fun v => Run (Call e1 (Value v)) l k))
 | SMakeCall : forall fname free arg l k body,
-        Forall value free ->
-        value arg ->
         nth_error E fname = Some body ->
-        sstep E (Run (Call (Close fname free) arg) l k)
+        sstep E (Run (Call (Value (Close fname free)) (Value arg)) l k)
                 (Run body (arg :: free) k)
-
 | SElimStepRec : forall rec cases l k,
-        ~ value rec ->
+        ~ is_value rec ->
         sstep E (Run (ElimBody rec cases) l k)
-                (Run rec l (fun v => Run (ElimBody v cases) l k))
+                (Run rec l (fun v => Run (ElimBody (Value v) cases) l k))
 | SEliminate : forall rec cases tag args l k case info e',
-        value rec ->
-        Forall value args ->
+        is_value rec ->
         nth_error cases tag = Some (case, info) ->
         unroll_elim rec case args info = Some e' ->
         sstep E (Run (ElimBody rec cases) (Constr tag args :: l) k)
@@ -96,33 +97,20 @@ Require Import Metadata.
 Definition prog_type : Type := list expr * list metadata.
 Definition valtype := HigherValue.value.
 
-Inductive expr_value : expr -> valtype -> Prop :=
-| EvConstr : forall tag args1 args2,
-        Forall2 expr_value args1 args2 ->
-        expr_value (Constr tag args1)
-                   (HigherValue.Constr tag args2)
-| EvClose : forall tag free1 free2,
-        Forall2 expr_value free1 free2 ->
-        expr_value (Close tag free1)
-                   (HigherValue.Close tag free2)
-.
 
 Inductive is_callstate (prog : prog_type) : valtype -> valtype -> state -> Prop :=
-| IsCallstate : forall fname free free_e av ae body,
+| IsCallstate : forall fname free av body,
         nth_error (fst prog) fname = Some body ->
         let fv := HigherValue.Close fname free in
-        expr_value ae av ->
-        Forall2 expr_value free_e free ->
         HigherValue.public_value (snd prog) fv ->
         HigherValue.public_value (snd prog) av ->
         is_callstate prog fv av
-            (Run body (ae :: free_e) Stop).
+            (Run body (av :: free) Stop).
 
 Inductive final_state (prog : prog_type) : state -> valtype -> Prop :=
-| FinalState : forall e v,
-        expr_value e v ->
+| FinalState : forall v,
         HigherValue.public_value (snd prog) v ->
-        final_state prog (Stop e) v.
+        final_state prog (Stop v) v.
 
 Definition initial_env (prog : prog_type) : env := fst prog.
 
@@ -131,35 +119,32 @@ Definition semantics (prog : prog_type) : Semantics.semantics :=
   @Semantics.Semantics_gen state env valtype
                  (is_callstate prog)
                  (sstep)
-                 (* (initial_state prog) *)
                  (final_state prog)
                  (initial_env prog).
 
+(* Lemma expr_value_value : forall e v, *)
+(*     expr_value e v -> *)
+(*     value e. *)
+(* induction e using expr_rect_mut with *)
+(*     (Pl := fun es => forall vs, *)
+(*         Forall2 expr_value es vs -> *)
+(*         Forall value es) *)
+(*     (Pp := fun e => forall v, *)
+(*         expr_value (fst e) v -> *)
+(*         value (fst e)) *)
+(*     (Plp := fun es => forall vs, *)
+(*         Forall2 (fun e v => expr_value (fst e) v) es vs -> *)
+(*         Forall (fun e => value (fst e)) es) ; *)
+(* intros0 Hev; try solve [invc Hev + simpl in *; eauto]. *)
 
+(* - invc Hev. constructor. eauto. *)
+(* - invc Hev. constructor. eauto. *)
+(* Qed. *)
+(* Hint Resolve expr_value_value. *)
 
-Lemma expr_value_value : forall e v,
-    expr_value e v ->
-    value e.
-induction e using expr_rect_mut with
-    (Pl := fun es => forall vs,
-        Forall2 expr_value es vs ->
-        Forall value es)
-    (Pp := fun e => forall v,
-        expr_value (fst e) v ->
-        value (fst e))
-    (Plp := fun es => forall vs,
-        Forall2 (fun e v => expr_value (fst e) v) es vs ->
-        Forall (fun e => value (fst e)) es) ;
-intros0 Hev; try solve [invc Hev + simpl in *; eauto].
-
-- invc Hev. constructor. eauto.
-- invc Hev. constructor. eauto.
-Qed.
-Hint Resolve expr_value_value.
-
-Lemma expr_value_value_list : forall e v,
-    Forall2 expr_value e v ->
-    Forall value e.
-induction e; intros0 Hev; invc Hev; eauto using expr_value_value.
-Qed.
-Hint Resolve expr_value_value_list.
+(* Lemma expr_value_value_list : forall e v, *)
+(*     Forall2 expr_value e v -> *)
+(*     Forall value e. *)
+(* induction e; intros0 Hev; invc Hev; eauto using expr_value_value. *)
+(* Qed. *)
+(* Hint Resolve expr_value_value_list. *)
