src/ElimFuncComp22.v
@@ -1,0 +1,941 @@
+Require Import Common Monads.
+Require Import Metadata.
+Require String.
+Require ElimFunc ElimFunc2.
+Require Import ListLemmas.
+Require Import StepLib.
+Require Import HigherValue.
+
+Require Import Psatz.
+
+Module A := ElimFunc.
+Module B := ElimFunc2.
+
+
+Fixpoint free_list' acc n :=
+    match n with
+    | 0 => B.Arg :: acc
+    | S n' => free_list' (B.UpVar n' :: acc) n'
+    end.
+
+Definition free_list n :=
+    match n with
+    | 0 => []
+    | S n => free_list' [] n
+    end.
+
+Definition close_dyn_free drop expect :=
+    skipn drop (free_list (expect + drop)).
+
+Definition compile :=
+    let fix go e :=
+        let fix go_list es :=
+            match es with
+            | [] => []
+            | e :: es => go e :: go_list es
+            end in
+        let fix go_pair p :=
+            let '(e, r) := p in (go e, r) in
+        let fix go_list_pair ps :=
+            match ps with
+            | [] => []
+            | p :: ps => go_pair p :: go_list_pair ps
+            end in
+        match e with
+        | A.Value v => B.Value v
+        | A.Arg => B.Arg
+        | A.UpVar n => B.UpVar n
+        | A.Call f a => B.Call (go f) (go a)
+        | A.MkConstr tag args => B.MkConstr tag (go_list args)
+        | A.ElimBody rec cases => B.ElimBody (go rec) (go_list_pair cases)
+        | A.MkClose fname free => B.MkClose fname (go_list free)
+        | A.MkCloseDyn fname drop expect => B.MkClose fname (close_dyn_free drop expect)
+        end in go.
+
+Definition compile_list :=
+    let go := compile in
+    let fix go_list es :=
+        match es with
+        | [] => []
+        | e :: es => go e :: go_list es
+        end in go_list.
+
+Definition compile_pair :=
+    let go := compile in
+    let fix go_pair (p : A.expr * A.rec_info) :=
+        let '(e, r) := p in (go e, r) in go_pair.
+
+Definition compile_list_pair :=
+    let go_pair := compile_pair in
+    let fix go_list_pair ps :=
+        match ps with
+        | [] => []
+        | p :: ps => go_pair p :: go_list_pair ps
+        end in go_list_pair.
+
+Ltac refold_compile :=
+    fold compile_list in *;
+    fold compile_pair in *;
+    fold compile_list_pair in *.
+
+
+Definition compile_func (f : A.expr) : option (B.expr) :=
+    if A.close_dyn_placement_dec f
+        then Some (compile f)
+        else None.
+
+Section compile_cu.
+Open Scope option_monad.
+
+Definition compile_cu (cu : list A.expr * list metadata) :
+        option (list B.expr * list metadata) :=
+    let '(funcs, metas) := cu in
+    map_partial compile_func funcs >>= fun funcs' =>
+    if B.enough_free_list_dec funcs' funcs'
+        then Some (funcs', metas)
+        else None.
+
+End compile_cu.
+
+
+Lemma compile_list_Forall : forall aes bes,
+    compile_list aes = bes ->
+    Forall2 (fun a b => compile a = b) aes bes.
+induction aes; destruct bes; intros0 Hcomp; simpl in Hcomp; try discriminate.
+- constructor.
+- invc Hcomp. eauto.
+Qed.
+
+Lemma compile_list_length : forall es,
+    length (compile_list es) = length es.
+intros. induction es.
+- reflexivity.
+- simpl. f_equal. eauto.
+Qed.
+
+Lemma compile_list_pair_length : forall es,
+    length (compile_list_pair es) = length es.
+intros. induction es.
+- reflexivity.
+- simpl. f_equal. eauto.
+Qed.
+
+
+
+Inductive I_expr (AE : A.env) (BE : B.env) : A.expr -> B.expr -> Prop :=
+| IValue :
+    forall v,
+      I_expr AE BE (A.Value v) (B.Value v)
+| IArg : I_expr AE BE A.Arg B.Arg
+| IUpVar : forall n, I_expr AE BE (A.UpVar n) (B.UpVar n)
+| ICall : forall af aa bf ba,
+        I_expr AE BE af bf ->
+        I_expr AE BE aa ba ->
+        I_expr AE BE (A.Call af aa) (B.Call bf ba)
+| IConstr : forall tag aargs bargs,
+        Forall2 (I_expr AE BE) aargs bargs ->
+        I_expr AE BE (A.MkConstr tag aargs) (B.MkConstr tag bargs)
+| IElimBody : forall arec acases brec bcases,
+        I_expr AE BE arec brec ->
+        Forall2 (fun ap bp => I_expr AE BE (fst ap) (fst bp) /\ snd ap = snd bp) acases bcases ->
+        I_expr AE BE (A.ElimBody arec acases) (B.ElimBody brec bcases)
+| IClose : forall fname afree bfree body,
+        nth_error BE fname = Some body ->
+        (* let n := length bfree in *)
+        (* B.num_locals body <= S n -> *)
+        (* n <= length afree -> *)
+        Forall2 (I_expr AE BE) afree bfree ->
+        (* Additional constraints ensure we avoid matching non-values to values.
+           This only matters after evaluating a CloseDyn, so it's okay. *)
+        (* Forall A.is_value (skipn n afree) -> *)
+        I_expr AE BE (A.MkClose fname afree) (B.MkClose fname bfree)
+| ICloseDyn : forall fname adrop aexpect bfree,
+        close_dyn_free adrop aexpect = bfree ->
+        I_expr AE BE (A.MkCloseDyn fname adrop aexpect)
+                     (B.MkClose fname bfree)
+.
+
+Inductive I (AE : A.env) (BE : B.env) : A.state -> B.state -> Prop :=
+| IRun : forall ae l ak be bk,
+        I_expr AE BE ae be ->
+        (forall v,
+            I AE BE (ak v) (bk v)) ->
+        I AE BE (A.Run ae l ak) (B.Run be l bk)
+
+(* Special hack for the intermediate state in `Call (CloseDyn _ _ 0) _`
+(* ### No longer happens, I believe *)
+   On the left, 2 steps:                      On the right, no steps:
+         Call (CloseDyn _ _ 0) _        <=>     Call (Close _ [])
+      -> CloseDyn _ _ 0  [k := ...]     <=>     ???
+      -> Call (Close _ []) _            <=>     Call (Close _ [])
+
+   This constructor handles the middle case.
+ *)
+(* | ICallCdz : forall fname drop aarg al ak barg bl bk, *)
+(*         I_expr AE BE aarg barg -> *)
+(*         Forall A.value al -> *)
+(*         Forall B.value bl -> *)
+(*         B.num_locals barg <= length bl -> *)
+(*         length bl <= length al -> *)
+(*         Forall2 (I_expr AE BE) (firstn (length bl) al) bl -> *)
+(*         (forall av bv, *)
+(*             A.value av -> *)
+(*             B.value bv -> *)
+(*             I_expr AE BE av bv -> *)
+(*             I AE BE (ak av) (bk bv)) -> *)
+(*         I AE BE (A.Run (A.CloseDyn fname drop 0) al *)
+(*                     (fun av => A.Run (A.Call av aarg) al ak)) *)
+(*                 (B.Run (B.Call (B.Close fname []) barg) bl bk) *)
+
+(* | IElimCdz : forall fname drop acases al ak bcases bl bk, *)
+(*         Forall2 (fun ap bp => I_expr AE BE (fst ap) (fst bp) /\ snd ap = snd bp) acases bcases -> *)
+(*         Forall A.value al -> *)
+(*         Forall B.value bl -> *)
+(*         S (B.num_locals_list_pair bcases) <= length bl -> *)
+(*         length bl <= length al -> *)
+(*         Forall2 (I_expr AE BE) (firstn (length bl) al) bl -> *)
+(*         (forall av bv, *)
+(*             A.value av -> *)
+(*             B.value bv -> *)
+(*             I_expr AE BE av bv -> *)
+(*             I AE BE (ak av) (bk bv)) -> *)
+(*         I AE BE (A.Run (A.CloseDyn fname drop 0) al *)
+(*                     (fun av => A.Run (A.ElimBody av acases) al ak)) *)
+(*                 (B.Run (B.ElimBody (B.Close fname []) bcases) bl bk) *)
+
+| IStop : forall v,
+        I AE BE (A.Stop v) (B.Stop v).
+
+
+
+(* `CloseDyn _ _ 0` needs all sorts of special handling, because it `compile`s
+ * from non-value to value (`Close _ []` is always a value) *)
+(* Inductive is_close_dyn_zero : A.expr -> Prop := *)
+(* | IsCloseDynZero : forall fname drop, is_close_dyn_zero (A.MkCloseDyn fname drop 0). *)
+
+(* Definition is_close_dyn_zero_dec (e : A.expr) : *)
+(*     { is_close_dyn_zero e } + { ~ is_close_dyn_zero e }. *)
+(* destruct e; try solve [right; inversion 1]. *)
+(* destruct expect; try solve [right; inversion 1]. *)
+(* left. constructor. *)
+(* Qed. *)
+
+(* Definition is_close_dyn_zero_state s := *)
+(*     match s with *)
+(*     | A.Run e _ _ => is_close_dyn_zero e *)
+(*     | A.Stop e => False *)
+(*     end. *)
+
+(*
+Inductive almost_value : A.expr -> Prop :=
+| AvConstr : forall tag args,
+        Forall almost_value args ->
+        almost_value (A.MkConstr tag args)
+| AvClose : forall fname free,
+        Forall almost_value free ->
+        almost_value (A.MkClose fname free)
+| AvCloseDynZero : forall fname drop,
+        almost_value (A.MkCloseDyn fname drop 0).
+
+Lemma value_almost_value : forall v, A.value v -> almost_value v.
+induction v using A.expr_ind''; inversion 1.
+- constructor. list_magic_on (args, tt).
+- constructor. list_magic_on (free, tt).
+Qed.
+
+*)
+
+Lemma free_list'_length : forall acc n,
+    length (free_list' acc n) = length acc + S n.
+first_induction n; intros.
+- simpl. lia.
+- simpl. rewrite IHn. simpl. lia.
+Qed.
+
+Lemma free_list_length : forall n, length (free_list n) = n.
+destruct n.
+- reflexivity.
+- eapply free_list'_length.
+Qed.
+
+Lemma close_dyn_free_length : forall drop expect,
+    length (close_dyn_free drop expect) = expect.
+intros. unfold close_dyn_free.
+rewrite skipn_length. rewrite free_list_length. lia.
+Qed.
+
+Lemma close_dyn_free_zero : forall drop, close_dyn_free drop 0 = [].
+intros.
+cut (length (close_dyn_free drop 0) = 0); [ | eapply close_dyn_free_length ].
+intro. destruct (close_dyn_free _ _); simpl in *.
+- reflexivity.
+- discriminate.
+Qed.
+
+
+Lemma compile_I_expr : forall AE BE ae be,
+    A.close_dyn_placement ae ->
+    B.enough_free BE be ->
+    compile ae = be ->
+    I_expr AE BE ae be.
+Proof.
+  intros AE BE.
+  induction ae using A.expr_rect_mut with
+  (Pl := fun aes => forall bes,
+             A.close_dyn_placement_list aes ->
+             B.enough_free_list BE bes ->
+             compile_list aes = bes ->
+             Forall2 (I_expr AE BE) aes bes)
+    (Pp := fun ap => forall bp,
+               A.close_dyn_placement_pair ap ->
+               B.enough_free_pair BE bp ->
+               compile_pair ap = bp ->
+               I_expr AE BE (fst ap) (fst bp) /\ snd ap = snd bp)
+    (Plp := fun aps => forall bps,
+                A.close_dyn_placement_list_pair aps ->
+                B.enough_free_list_pair BE bps ->
+                compile_list_pair aps = bps ->
+                Forall2 (fun ap bp => I_expr AE BE (fst ap) (fst bp) /\ snd ap = snd bp) aps bps);
+    intros0 Hcdp Hfree Hcomp;
+    simpl in Hcomp; refold_compile; try rewrite <- Hcomp; try rewrite <- Hcomp in Hfree;
+      simpl in Hfree; B.refold_enough_free BE; repeat (break_exists || break_and);
+        invc Hcdp || simpl in Hcdp; try solve [eauto | constructor; eauto].
+
+  (* Call case *)
+  - destruct ae1; try invc Hcdp; try solve [constructor; eauto; constructor; eauto].
+
+  (* ElimBody case *)
+  - A.refold_close_dyn_placement.
+    destruct ae; break_and; try on (A.close_dyn_placement _), invc;
+      try solve [constructor; eauto; constructor; eauto].
+
+  (* Close case *)
+  - rename x into body. A.refold_close_dyn_placement.
+    rewrite compile_list_length in *.
+    econstructor; eauto.
+    (* + rewrite compile_list_length. auto. *)
+    (* + rewrite compile_list_length. lia. *)
+    (* + rewrite compile_list_length. rewrite firstn_all by auto. eapply IHae; eauto. *)
+    (* + remember (skipn _ _) as free'. *)
+    (*   assert (length free' = 0). *)
+    (*   { subst free'. rewrite skipn_length. rewrite compile_list_length. lia. } *)
+    (*   destruct free'; try discriminate. *)
+    (*   constructor. *)
+Qed.
+
+(* Lemma compile_func_close_dyn_placement : forall a b, *)
+(*     compile_func a = Some b -> *)
+(*     A.close_dyn_placement a. *)
+(* intros0 Hcomp. *)
+(* unfold compile_func in Hcomp. break_if; try discriminate. inject_some. *)
+(* auto. *)
+(* Qed. *)
+
+(* Theorem compile_cu_close_dyn_placement : forall a ameta b bmeta, *)
+(*     compile_cu (a, ameta) = Some (b, bmeta) -> *)
+(*     Forall A.close_dyn_placement a. *)
+(* intros0 Hcomp. unfold compile_cu in *. break_bind_option. *)
+(*   break_if; try discriminate. inject_some. *)
+(* on _, apply_lem map_partial_Forall2. *)
+(* list_magic_on (a, (b, tt)). eauto using compile_func_close_dyn_placement. *)
+(* Qed. *)
+
+(* Theorem compile_cu_enough_free : forall a ameta b bmeta, *)
+(*     compile_cu (a, ameta) = Some (b, bmeta) -> *)
+(*     Forall (B.enough_free b) b. *)
+(* intros0 Hcomp. unfold compile_cu in *. break_bind_option. *)
+(*   break_if; try discriminate. inject_some. *)
+(* rewrite <- B.enough_free_list_Forall. auto. *)
+(* Qed. *)
+
+(* Definition var_n n := *)
+(*     match n with *)
+(*     | 0 => B.Arg *)
+(*     | S n' => B.UpVar n' *)
+(*     end. *)
+
+(* Lemma free_list'_nth_error : forall acc n i, *)
+(*     (forall j, j < length acc -> *)
+(*         nth_error acc j = Some (var_n (S n + j))) -> *)
+(*     i < length acc + S n -> *)
+(*     nth_error (free_list' acc n) i = Some (var_n i). *)
+(* first_induction n; intros0 Hacc Hlt; simpl. *)
+(* - destruct i. *)
+(*   + simpl. reflexivity. *)
+(*   + simpl. rewrite Hacc by lia. simpl. reflexivity. *)
+(* - rewrite IHn; [ eauto | | simpl; lia ]. *)
+(*   intros. simpl in *. *)
+(*   destruct j; simpl. *)
+(*   + replace (n + 0) with n by lia. reflexivity. *)
+(*   + rewrite Hacc by lia. do 2 f_equal. lia. *)
+(* Qed. *)
+
+(* Lemma free_list_nth_error : forall n i, *)
+(*     i < n -> *)
+(*     nth_error (free_list n) i = Some (var_n i). *)
+(* intros0 Hlt. *)
+(* destruct n. *)
+(*   { lia. } *)
+(* simpl. rewrite free_list'_nth_error; eauto. *)
+(* simpl. intros. lia. *)
+(* Qed. *)
+
+(* Lemma close_dyn_free_nth_error : forall drop expect i, *)
+(*     i < expect -> *)
+(*     nth_error (close_dyn_free drop expect) i = Some (var_n (drop + i)). *)
+(* intros0 Hlt. *)
+(* unfold close_dyn_free. *)
+(* rewrite skipn_nth_error. rewrite free_list_nth_error by lia. *)
+(* reflexivity. *)
+(* Qed. *)
+
+(* Lemma var_n_num_locals : forall n, B.num_locals (var_n n) = S n. *)
+(* destruct n; simpl; reflexivity. *)
+(* Qed. *)
+
+(* Lemma close_dyn_free_num_locals : forall expect drop, *)
+(*     0 < expect -> *)
+(*     B.num_locals_list (close_dyn_free drop expect) = drop + expect. *)
+(* intros0 Hlt. *)
+
+(* rewrite B.num_locals_list_is_maximum. *)
+(* fwd eapply close_dyn_free_length with (drop := drop) (expect := expect). *)
+(* remember (close_dyn_free _ _) as free. *)
+
+(* assert (maximum (map B.num_locals free) <= drop + expect). { *)
+(*     rewrite maximum_le_Forall. rewrite <- Forall_map. *)
+(*     rewrite Forall_forall. intros0 Hin. *)
+(*     eapply In_nth_error in Hin. break_exists. *)
+(*     assert (x0 < expect). { *)
+(*       erewrite <- close_dyn_free_length with (drop := drop). *)
+(*       rewrite <- nth_error_Some. congruence. *)
+(*     } *)
+(*     subst free. rewrite close_dyn_free_nth_error in * by assumption. *)
+(*     inject_some. rewrite var_n_num_locals. *)
+(*     lia. *)
+(* } *)
+
+(* assert (maximum (map B.num_locals free) >= drop + expect). { *)
+(*     replace free with (slice 0 expect free); cycle 1. *)
+(*       { unfold slice. simpl. rewrite firstn_all by lia. reflexivity. } *)
+(*     rewrite slice_split with (k := expect - 1) by lia. *)
+(*     rewrite map_app. rewrite maximum_app. *)
+(*     replace (expect) with (S (expect - 1)) at 3 by lia. *)
+(*     erewrite nth_error_slice; cycle 1. *)
+(*       { subst free. eapply close_dyn_free_nth_error. lia. } *)
+(*     simpl. rewrite var_n_num_locals. *)
+(*     lia. *)
+(* } *)
+
+(* lia. *)
+(* Qed. *)
+
+(* Lemma slice_all : forall A (xs : list A), *)
+(*     slice 0 (length xs) xs = xs. *)
+(* intros. unfold slice. simpl. rewrite firstn_all by lia. reflexivity. *)
+(* Qed. *)
+
+(*
+Ltac B_start HS :=
+    match goal with
+    | [ |- context [ ?pred ?E ?s _ ] ] =>
+            lazymatch pred with
+            | B.sstep => idtac
+            | B.sstar => idtac
+            | B.splus => idtac
+            | _ => fail "unrecognized predicate:" pred
+            end;
+            let S_ := fresh "S" in
+            let S0 := fresh "S" in
+            set (S0 := s);
+            change s with S0;
+            assert (HS : B.sstar E S0 S0) by (eapply B.SStarNil)
+    end.
+
+Ltac B_step HS :=
+    let S_ := fresh "S" in
+    let S2 := fresh "S" in
+    let HS' := fresh HS "'" in
+    let go E s0 s1 Brel solver :=
+        rename HS into HS';
+        evar (S2 : B.state);
+        assert (HS : Brel E s0 S2);
+        [ solver; unfold S2
+        | clear HS' ] in
+    match type of HS with
+    | B.sstar ?E ?s0 ?s1 => go E s0 s1 B.splus
+            ltac:(eapply sstar_then_splus with (1 := HS');
+                  eapply B.SPlusOne)
+    | B.splus ?E ?s0 ?s1 => go E s0 s1 B.splus
+            ltac:(eapply splus_snoc with (1 := HS'))
+    end.
+
+Ltac B_star HS :=
+    let S_ := fresh "S" in
+    let S2 := fresh "S" in
+    let HS' := fresh HS "'" in
+    let go E s0 s1 Brel solver :=
+        rename HS into HS';
+        evar (S2 : B.state);
+        assert (HS : Brel E s0 S2);
+        [ solver; unfold S2
+        | clear HS' ] in
+    match type of HS with
+    | B.sstar ?E ?s0 ?s1 => go E s0 s1 B.sstar
+            ltac:(eapply sstar_then_sstar with (1 := HS'))
+    | B.splus ?E ?s0 ?s1 => go E s0 s1 B.splus
+            ltac:(eapply splus_then_sstar with (1 := HS'))
+    end.
+
+Ltac B_plus HS :=
+    let S_ := fresh "S" in
+    let S2 := fresh "S" in
+    let HS' := fresh HS "'" in
+    let go E s0 s1 Brel solver :=
+        rename HS into HS';
+        evar (S2 : B.state);
+        assert (HS : Brel E s0 S2);
+        [ solver; unfold S2
+        | clear HS' ] in
+    match type of HS with
+    | B.sstar ?E ?s0 ?s1 => go E s0 s1 B.splus
+            ltac:(eapply sstar_then_splus with (1 := HS'))
+    | B.splus ?E ?s0 ?s1 => go E s0 s1 B.splus
+            ltac:(eapply splus_then_splus with (1 := HS'))
+    end.
+*)
+
+
+
+(* Lemma nth_error_Some_ex : forall A (xs : list A) n, *)
+(*     n < length xs -> *)
+(*     exists x, nth_error xs n = Some x. *)
+(* Proof. *)
+(*   intros0 Hlen. rewrite <- nth_error_Some in Hlen. *)
+(*   destruct (nth_error _ _) eqn:?; try congruence. *)
+(*   eauto. *)
+(* Qed. *)
+
+(*
+Definition count_close_dyn_zero :=
+    let fix go e :=
+        let fix go_list es :=
+            match es with
+            | [] => 0
+            | e :: es => go e + go_list es
+            end in
+        let fix go_pair p :=
+            match p with
+            | (e, _) => go e
+            end in
+        let fix go_list_pair ps :=
+            match ps with
+            | [] => 0
+            | p :: ps => go_pair p + go_list_pair ps
+            end in
+        match e with
+        | A.Arg => 0
+        | A.UpVar _ => 0
+        | A.Call f a => go f + go a
+        | A.Constr _ args => go_list args
+        | A.ElimBody rec cases => go rec + go_list_pair cases
+        | A.Close _ free => go_list free
+        | A.CloseDyn _ _ 0 => 1
+        | A.CloseDyn _ _ _ => 0
+        end in go.
+
+Definition count_close_dyn_zero_list :=
+    let go := count_close_dyn_zero in
+    let fix go_list es :=
+        match es with
+        | [] => 0
+        | e :: es => go e + go_list es
+        end in go_list.
+
+Definition count_close_dyn_zero_pair :=
+    let go := count_close_dyn_zero in
+    let fix go_pair (p : A.expr * A.rec_info) :=
+        match p with
+        | (e, _) => go e
+        end in go_pair.
+
+Definition count_close_dyn_zero_list_pair :=
+    let go_pair := count_close_dyn_zero_pair in
+    let fix go_list_pair ps :=
+        match ps with
+        | [] => 0
+        | p :: ps => go_pair p + go_list_pair ps
+        end in go_list_pair.
+
+Ltac refold_count_close_dyn_zero :=
+    fold count_close_dyn_zero_list in *;
+    fold count_close_dyn_zero_pair in *;
+    fold count_close_dyn_zero_list_pair in *.
+
+Definition count_close_dyn_zero_state s :=
+    match s with
+    | A.Run e _ _ => count_close_dyn_zero e
+    | A.Stop e => count_close_dyn_zero e
+    end.
+
+Lemma value_count_close_dyn_zero : forall e,
+    A.value e ->
+    count_close_dyn_zero e = 0.
+induction e using A.expr_rect_mut with
+    (Pl := fun es =>
+        Forall A.value es ->
+        count_close_dyn_zero_list es = 0)
+    (Pp := fun p =>
+        A.value (fst p) ->
+        count_close_dyn_zero_pair p = 0)
+    (Plp := fun ps =>
+        Forall (fun p => A.value (fst p)) ps ->
+        count_close_dyn_zero_list_pair ps = 0);
+inversion 1; simpl; refold_count_close_dyn_zero; eauto.
+all: rewrite (IHe ** ).
+all: rewrite (IHe0 ** ).
+all: reflexivity.
+Qed.
+
+Lemma value_count_close_dyn_zero_list : forall es,
+    Forall A.value es ->
+    count_close_dyn_zero_list es = 0.
+induction es; inversion 1; simpl; refold_count_close_dyn_zero.
+- reflexivity.
+- rewrite value_count_close_dyn_zero by assumption.
+  rewrite IHes by assumption.
+  reflexivity.
+Qed.
+*)
+
+(*
+Definition A_value_dec : forall e : A.expr, { A.value e } + { ~ A.value e }.
+induction e using A.expr_rect_mut with
+    (Pl := fun es => { Forall A.value es } + { ~ Forall A.value es })
+    (Pp := fun p => { A.value (fst p) } + { ~ A.value (fst p) })
+    (Plp := fun ps => { Forall (fun p => A.value (fst p)) ps } +
+                      { ~ Forall (fun p => A.value (fst p)) ps });
+try solve [left; constructor | right; inversion 1].
+
+- (* constr *)
+  destruct IHe; [ | right; inversion 1; eauto ].
+  left. constructor. eauto.
+
+- (* close *)
+  destruct IHe; [ | right; inversion 1; eauto ].
+  left. constructor. eauto.
+
+- (* cons *)
+  destruct IHe; [ | right; inversion 1; eauto ].
+  destruct IHe0; [ | right; inversion 1; eauto ].
+  left. constructor; eauto.
+
+- (* pair *)
+  simpl. assumption.
+
+- (* cons *)
+  destruct IHe; [ | right; inversion 1; eauto ].
+  destruct IHe0; [ | right; inversion 1; eauto ].
+  left. constructor; eauto.
+Defined.
+ *)
+
+(* Definition A_rec_info_eq_dec (x y : A.rec_info) : { x = y } + { x <> y }. *)
+(*   decide equality. decide equality. *)
+(* Defined. *)
+
+(*
+Definition A_expr_eq_dec (x y : A.expr) : { x = y } + { x <> y }.
+generalize dependent y.
+induction x using A.expr_rect_mut with
+    (Pl := fun es => forall es', { es = es' } + { es <> es' })
+    (Pp := fun p => forall p', { p = p' } + { p <> p' })
+    (Plp := fun ps => forall ps', { ps = ps' } + { ps <> ps' });
+intros.
+
+
+- destruct y; try (right; congruence).
+  left. congruence.
+
+- destruct y; try (right; congruence).
+  destruct (eq_nat_dec n n0); try (right; congruence).
+  left. congruence.
+
+- destruct y; try (right; congruence).
+  destruct (IHx1 y1); try (right; congruence).
+  destruct (IHx2 y2); try (right; congruence).
+  left. congruence.
+
+- destruct y; try (right; congruence).
+  destruct (eq_nat_dec tag tag0); try (right; congruence).
+  destruct (IHx args0); try (right; congruence).
+  left. congruence.
+
+- destruct y; try (right; congruence).
+  destruct (IHx y); try (right; congruence).
+  destruct (IHx0 cases0); try (right; congruence).
+  left. congruence.
+
+- destruct y; try (right; congruence).
+  destruct (eq_nat_dec f f0); try (right; congruence).
+  destruct (IHx free0); try (right; congruence).
+  left. congruence.
+
+- destruct y; try (right; congruence).
+  destruct (eq_nat_dec f f0); try (right; congruence).
+  destruct (eq_nat_dec drop drop0); try (right; congruence).
+  destruct (eq_nat_dec expect expect0); try (right; congruence).
+  left. congruence.
+
+
+- destruct es'; try (right; congruence).
+  left. congruence.
+
+- destruct es'; try (right; congruence).
+  destruct (IHx e); try (right; congruence).
+  destruct (IHx0 es'); try (right; congruence).
+  left. congruence.
+
+
+- destruct p'; try (right; congruence).
+  destruct (IHx e); try (right; congruence).
+  destruct (A_rec_info_eq_dec r r0); try (right; congruence).
+  left. congruence.
+
+
+- destruct ps'; try (right; congruence).
+  left. congruence.
+
+- destruct ps'; try (right; congruence).
+  destruct (IHx p0); try (right; congruence).
+  destruct (IHx0 ps'); try (right; congruence).
+  left. congruence.
+Defined.
+*)
+
+(*Definition A_matchable s := ~ is_close_dyn_zero_state s.*)
+
+
+(* Lemma compile_num_locals : forall a b, *)
+(*     compile a = b -> *)
+(*     A.num_locals a = B.num_locals b. *)
+(* Proof. *)
+(* induction a using A.expr_rect_mut with *)
+(*     (Pl := fun a => forall b, *)
+(*         compile_list a = b -> *)
+(*         A.num_locals_list a = B.num_locals_list b) *)
+(*     (Pp := fun a => forall b, *)
+(*         compile_pair a = b -> *)
+(*         A.num_locals_pair a = B.num_locals_pair b) *)
+(*     (Plp := fun a => forall b, *)
+(*         compile_list_pair a = b -> *)
+(*         A.num_locals_list_pair a = B.num_locals_list_pair b); *)
+(* intros0 Hcomp; *)
+(* simpl in *; refold_compile; A.refold_num_locals; *)
+(* subst; simpl; B.refold_num_locals. *)
+
+(* - reflexivity. *)
+(* - reflexivity. *)
+(* - reflexivity. *)
+(* - erewrite IHa1, IHa2; reflexivity. *)
+(* - erewrite IHa; reflexivity. *)
+(* - erewrite IHa, IHa0; reflexivity. *)
+(* - erewrite IHa; reflexivity. *)
+(* - break_if. *)
+(*   + subst. rewrite close_dyn_free_zero. reflexivity. *)
+(*   + rewrite close_dyn_free_num_locals by lia. reflexivity. *)
+
+(* - reflexivity. *)
+(* - erewrite IHa, IHa0; reflexivity. *)
+
+(* - eauto. *)
+
+(* - reflexivity. *)
+(* - erewrite IHa, IHa0; reflexivity. *)
+(* Qed. *)
+
+(*Lemma I_sim :
+  forall AE BE a a' b,
+    compile_list AE = BE ->
+    Forall A.close_dyn_placement AE ->
+    Forall (B.enough_free BE) BE ->
+    I AE BE a b ->
+    A.sstep AE a a' ->
+    B.enough_free_state BE b ->
+    exists b',
+        (B.splus BE b b' \/
+         (b' = b /\ state_metric a' < state_metric a)) /\
+        I AE BE a' b'.*)
+
+
+Lemma MkCloseDyn_step_sim :
+  forall expect drop l AE f  ak bk,
+    A.sstep AE (A.Run (A.MkCloseDyn f drop expect) l ak) (ak (Close f (skipn drop l))) ->
+    I_expr AE (compile_list AE) (A.MkCloseDyn f drop expect) (B.MkClose f (close_dyn_free drop expect)) ->
+    (forall v, I AE (compile_list AE) (ak v) (bk v)) ->
+    drop >= length l ->
+    exists b',
+      B.splus (compile_list AE) (B.Run (B.MkClose f (close_dyn_free drop expect)) l bk) b' /\
+      I AE (compile_list AE) (ak (Close f (skipn drop l))) b'.
+Proof.
+  induction expect; intros.
+  eexists; split.
+  rewrite close_dyn_free_zero in *.
+  eapply SPlusOne.
+  replace ([]) with (map B.Value []) by reflexivity.
+  econstructor.
+  replace (skipn drop l) with (@nil value).
+  eapply H1. rewrite skipn_all; try omega; eauto.
+  
+  (* We need to know that (skipn drop l) is [] *)
+  (* We could do that by knowing that expect + drop = length l *)
+  (* TODO: add this to I or I_expr *)
+
+  
+  
+Admitted.
+  
+Lemma I_sim :
+  forall AE BE a a' b,
+    compile_list AE = BE ->
+    I AE BE a b ->
+    A.sstep AE a a' ->
+    exists b',
+      B.splus BE b b' /\
+      I AE BE a' b'.
+Proof.
+  destruct a as [ae al ak | ae];
+    intros; [ | solve [on (A.sstep _ _ _), inv] ].
+
+  destruct ae; on (A.sstep _ _ _),  inv; on (I _ _ _ _), invc; [ try on (I_expr _ _ _ _), invc.. | | ].
+  
+  Focus 12.
+  on (I_expr _ _ _ _), inv.
+  eapply MkCloseDyn_step_sim.
+  
+  
+  
+Admitted.
+
+Definition match_values (AE : A.env) (BE : B.env) (M : list metadata) : value -> value -> Prop := eq.
+
+Ltac i_ctor := intros; econstructor; eauto.
+Ltac i_lem H := intros; eapply H; eauto.
+
+(* Lemma match_values_public : forall A B M bv av, *)
+(*     match_values A B M av bv -> *)
+(*     public_value M bv -> *)
+(*     public_value M av. *)
+(* intros until M. *)
+(* mut_induction bv using value_rect_mut' with *)
+(*     (Pl := fun bv => forall av, *)
+(*         Forall2 (match_values A B M) av bv -> *)
+(*         Forall (public_value M) bv -> *)
+(*         Forall (public_value M) av); *)
+(* [ intros0 Hmv Bpub; invc Hmv; invc Bpub; i_ctor.. | ]. *)
+(* - finish_mut_induction match_values_public using list. *)
+(* Qed exporting. *)
+
+Lemma compile_cu_compile_list : forall a ameta b bmeta,
+    compile_cu (a, ameta) = Some (b, bmeta) ->
+    compile_list a = b.
+intros.
+simpl in *. break_bind_option. break_if; try discriminate. inject_some.
+on _, apply_lem map_partial_Forall2.
+on >B.enough_free_list, fun H => clear H.
+generalize dependent b. induction a; intros; on >Forall2, invc.
+- simpl. reflexivity.
+- simpl. f_equal; eauto.
+  unfold compile_func in *. break_if; try discriminate. inject_some. reflexivity.
+Qed.
+
+Section Preservation.
+
+  Variable prog : A.prog_type.
+  Variable tprog : B.prog_type.
+
+  Hypothesis TRANSF : compile_cu prog = Some tprog.
+
+  Theorem fsim :
+    Semantics.forward_simulation (A.semantics prog) (B.semantics tprog).
+  Proof.
+    destruct prog as [A Ameta], tprog as [B Bmeta].
+    (* fwd eapply compile_cu_close_dyn_placement; eauto. *)
+    (* fwd eapply compile_cu_enough_free; eauto. *)
+    (* fwd eapply compile_cu_Forall; eauto. *)
+    (* fwd eapply compile_cu_metas; eauto. *)
+
+    eapply Semantics.forward_simulation_step with
+        (match_states := I A B)
+        (match_values := match_values A B Ameta).
+
+    - simpl. intros. on >B.is_callstate, invc. simpl in *.
+      admit.
+      
+      (* fwd eapply Forall2_nth_error_ex' with (xs := A) (ys := B) as HH; eauto. *)
+      (*   destruct HH as (abody & ? & ?). *)
+
+      (* fwd eapply match_values_I_expr with (bv := av2) as HH; eauto. *)
+      (*   destruct HH as (av1_e & ? & ?). *)
+      (* on (match_values _ _ _ _ (Close _ _)), invc. *)
+      (* fwd eapply match_values_I_expr_list with (avs := afree) as HH; eauto. *)
+      (*   destruct HH as (afree_e & ? & ?). *)
+
+      (* eexists. split. 1: econstructor. *)
+      (* + econstructor. *)
+      (*   * i_lem compile_I_expr; i_lem Forall_nth_error. *)
+      (*   * instantiate (1 := av1_e :: afree_e). *)
+      (*     eauto using A.expr_value_value_list. *)
+      (*   * eauto using B.expr_value_value, B.expr_value_value_list. *)
+      (*   * simpl. subst n. collect_length_hyps. congruence. *)
+      (*   * simpl. collect_length_hyps. *)
+      (*     rewrite firstn_length, min_l in * by auto. omega. *)
+      (*   * simpl. i_ctor. *)
+      (*     collect_length_hyps. subst n. congruence. *)
+      (*   * i_ctor. *)
+
+
+      (* + i_ctor. *)
+      (*   * i_lem Forall_nth_error. *)
+      (*   * constructor. *)
+      (*     -- eapply match_values_enough_free; [ | | eassumption ]; eauto. *)
+      (*     -- eapply match_values_enough_free_list; eauto. *)
+      (*   * i_ctor. *)
+
+      (* + i_ctor. *)
+      (*   * on (public_value _ (Close _ _)), invc. i_ctor. *)
+      (*   * i_lem match_values_public. *)
+
+    - intros0 II Afinal. invc Afinal.
+      invc II.
+
+      eexists.
+      split.
+      i_ctor.
+      simpl in H. simpl.
+      
+      admit.
+      reflexivity.
+
+    - intros0 Astep. intros0 II.
+      eapply I_sim; try eassumption.
+      + eapply compile_cu_compile_list; eauto.
+        
+  Admitted.
+  (* Defined. *)
+
+  (*   Lemma match_val_eq : *)
+  (*     Semantics.fsim_match_val _ _ fsim = match_values (fst prog) (fst tprog) (snd prog). *)
+  (*   Proof. *)
+  (*     unfold fsim. simpl. *)
+  (*     unfold Semantics.fsim_match_val. *)
+  (*     break_match. repeat (break_match_hyp; try congruence). *)
+  (*     try unfold forward_simulation_step in *. *)
+  (*     try unfold forward_simulation_plus in *. *)
+  (*     try unfold forward_simulation_star in *. *)
+  (*     try unfold forward_simulation_star_wf in *. *)
+  (*     inv Heqf. reflexivity. *)
+  (* Qed. *)
+
+End Preservation.
+    
